case_study/RiscvPmp/IrisModelBinary.v
@@ -1,0 +1,155 @@
+(******************************************************************************)
+(* Copyright (c) 2020 Steven Keuchel, Dominique Devriese, Sander Huyghebaert  *)
+(* All rights reserved.                                                       *)
+(*                                                                            *)
+(* Redistribution and use in source and binary forms, with or without         *)
+(* modification, are permitted provided that the following conditions are     *)
+(* met:                                                                       *)
+(*                                                                            *)
+(* 1. Redistributions of source code must retain the above copyright notice,  *)
+(*    this list of conditions and the following disclaimer.                   *)
+(*                                                                            *)
+(* 2. Redistributions in binary form must reproduce the above copyright       *)
+(*    notice, this list of conditions and the following disclaimer in the     *)
+(*    documentation and/or other materials provided with the distribution.    *)
+(*                                                                            *)
+(* THIS SOFTWARE IS PROVIDED BY THE COPYRIGHT HOLDERS AND CONTRIBUTORS        *)
+(* "AS IS" AND ANY EXPRESS OR IMPLIED WARRANTIES, INCLUDING, BUT NOT LIMITED  *)
+(* TO, THE IMPLIED WARRANTIES OF MERCHANTABILITY AND FITNESS FOR A PARTICULAR *)
+(* PURPOSE ARE DISCLAIMED. IN NO EVENT SHALL THE COPYRIGHT HOLDER OR          *)
+(* CONTRIBUTORS BE LIABLE FOR ANY DIRECT, INDIRECT, INCIDENTAL, SPECIAL,      *)
+(* EXEMPLARY, OR CONSEQUENTIAL DAMAGES (INCLUDING, BUT NOT LIMITED TO,        *)
+(* PROCUREMENT OF SUBSTITUTE GOODS OR SERVICES; LOSS OF USE, DATA, OR         *)
+(* PROFITS; OR BUSINESS INTERRUPTION) HOWEVER CAUSED AND ON ANY THEORY OF     *)
+(* LIABILITY, WHETHER IN CONTRACT, STRICT LIABILITY, OR TORT (INCLUDING       *)
+(* NEGLIGENCE OR OTHERWISE) ARISING IN ANY WAY OUT OF THE USE OF THIS         *)
+(* SOFTWARE, EVEN IF ADVISED OF THE POSSIBILITY OF SUCH DAMAGE.               *)
+(******************************************************************************)
+
+From Katamaran Require Import
+     Bitvector
+     Environment
+     Iris.Model
+     Iris.BinaryWp
+     Iris.BinaryInstance
+     RiscvPmp.Machine
+     RiscvPmp.IrisModel.
+From iris Require Import
+     base_logic.lib.gen_heap
+     proofmode.tactics.
+
+Set Implicit Arguments.
+
+Import RiscvPmpProgram.
+
+(* Instantiate the Iris framework solely using the operational semantics. At
+   this point we do not commit to a set of contracts nor to a set of
+   user-defined predicates. *)
+Module RiscvPmpIrisBase2 <: IrisBase2 RiscvPmpBase RiscvPmpProgram RiscvPmpSemantics.
+  (* Pull in the definition of the LanguageMixin and register ghost state. *)
+  Include IrisPrelims RiscvPmpBase RiscvPmpProgram RiscvPmpSemantics.
+
+  (* Defines the memory ghost state. *)
+  Section RiscvPmpIrisParams2.
+    Import bv.
+    Definition Byte : Set := bv 8.
+    Definition MemVal : Set := Byte.
+
+    Class mcMemGS2 Σ :=
+      McMemGS2 {
+          (* ghost variable for tracking state of registers *)
+          mc_ghGS2 : gen_heapGS Addr (MemVal * MemVal) Σ
+        }.
+    #[export] Existing Instance mc_ghGS2.
+
+    Definition memGpreS2 : gFunctors -> Set := fun Σ => gen_heapGpreS Addr (MemVal * MemVal) Σ.
+    Definition memGS2 : gFunctors -> Set := mcMemGS2.
+    Definition memΣ2 : gFunctors := gen_heapΣ Addr (MemVal * MemVal).
+
+    Definition liveAddrs := bv.seqBv (@bv.of_nat xlenbits minAddr) lenAddr.
+    Lemma NoDup_liveAddrs : NoDup liveAddrs.
+    Proof. now eapply Prelude.nodup_fixed. Qed.
+
+    #[global] Arguments liveAddrs : simpl never.
+
+    Definition initMemMap2 μ1 μ2 := (list_to_map (map (fun a => (a , (μ1 a , μ2 a))) liveAddrs) : gmap Addr (MemVal * MemVal)).
+
+    Definition memΣ_GpreS2 : forall {Σ}, subG memΣ2 Σ -> memGpreS2 Σ :=
+      fun {Σ} => subG_gen_heapGpreS (Σ := Σ) (L := Addr) (V := MemVal * MemVal).
+
+    Definition mem_inv2 : forall {Σ}, mcMemGS2 Σ -> Memory -> Memory -> iProp Σ :=
+      fun {Σ} hG μ1 μ2 =>
+        (∃ memmap, gen_heap_interp memmap ∗
+           ⌜ map_Forall (fun a v => (μ1 a , μ2 a) = v) memmap ⌝
+        )%I.
+
+    Definition mem_res2 `{hG : mcMemGS2 Σ} : Memory -> Memory -> iProp Σ :=
+      fun μ1 μ2 => ([∗ list] a' ∈ liveAddrs, mapsto a' (DfracOwn 1) (μ1 a' , μ2 a'))%I.
+
+    Lemma initMemMap2_works μ1 μ2 : map_Forall (λ (a : Addr) (v : MemVal * MemVal), (μ1 a , μ2 a) = v) (initMemMap2 μ1 μ2).
+    Proof.
+      unfold initMemMap2.
+      rewrite map_Forall_to_list.
+      rewrite Forall_forall.
+      intros (a , v).
+      rewrite elem_of_map_to_list.
+      intros el.
+      apply elem_of_list_to_map_2 in el.
+      apply elem_of_list_In in el.
+      apply in_map_iff in el.
+      by destruct el as (a' & <- & _).
+    Qed.
+
+    Lemma mem_inv_init2 `{gHP : memGpreS2 Σ} (μ1 μ2 : Memory) :
+      ⊢ |==> ∃ mG : mcMemGS2 Σ, (mem_inv2 mG μ1 μ2 ∗ mem_res2 μ1 μ2)%I.
+    Proof.
+      iMod (gen_heap_init (gen_heapGpreS0 := gHP) (L := Addr) (V := MemVal * MemVal) empty) as (gH) "[inv _]".
+
+      pose (memmap := initMemMap2 μ1 μ2).
+      iMod (gen_heap_alloc_big empty memmap (map_disjoint_empty_r memmap) with "inv") as "(inv & res & _)".
+      iModIntro.
+
+      rewrite (right_id empty union memmap).
+
+      iExists (McMemGS2 gH).
+      iSplitL "inv".
+      - iExists memmap.
+        iFrame.
+        iPureIntro.
+        apply initMemMap2_works.
+      - unfold mem_res2, initMemMap2 in *.
+        iApply (RiscvPmpIrisBase.big_sepM_list_to_map (f := fun a => (μ1 a , μ2 a)) (fun a v => mapsto a (DfracOwn 1) v) with "[$]").
+        eapply NoDup_liveAddrs.
+    Qed.
+
+    (* Note: this defaultRegStore is only needed for technical reason, it is not used. *)
+    Definition defaultRegStore : RegStore :=
+      fun τ r =>
+        match r with
+          pc => (bv.zero : TypeDecl.ty.Val ty_xlenbits)
+        | nextpc => (bv.zero : TypeDecl.ty.Val ty_xlenbits)
+        | mstatus => (MkMstatus Machine : TypeDecl.ty.Val ty_mstatus)
+        | mtvec => (bv.zero : TypeDecl.ty.Val ty_xlenbits)
+        | mcause => (bv.zero : TypeDecl.ty.Val ty_xlenbits)
+        | mepc => (bv.zero : TypeDecl.ty.Val ty_xlenbits)
+        | cur_privilege => Machine
+        | x1 => (bv.zero : TypeDecl.ty.Val ty_xlenbits)
+        | x2 => (bv.zero : TypeDecl.ty.Val ty_xlenbits)
+        | x3 => (bv.zero : TypeDecl.ty.Val ty_xlenbits)
+        | x4 => (bv.zero : TypeDecl.ty.Val ty_xlenbits)
+        | x5 => (bv.zero : TypeDecl.ty.Val ty_xlenbits)
+        | x6 => (bv.zero : TypeDecl.ty.Val ty_xlenbits)
+        | x7 => (bv.zero : TypeDecl.ty.Val ty_xlenbits)
+        | pmp0cfg => (MkPmpcfg_ent false OFF true true true : TypeDecl.ty.Val ty_pmpcfg_ent)
+        | pmp1cfg => (MkPmpcfg_ent false OFF true true true : TypeDecl.ty.Val ty_pmpcfg_ent)
+        | pmpaddr0 => (bv.zero : TypeDecl.ty.Val ty_xlenbits)
+        | pmpaddr1 => (bv.zero : TypeDecl.ty.Val ty_xlenbits)
+        end.
+
+    (* Note: this defaultMemory is only needed for technical reason, it is not used. *)
+    Definition defaultMemory : Memory := fun a => bv.zero.
+  End RiscvPmpIrisParams2.
+
+  Include IrisResources2 RiscvPmpBase RiscvPmpProgram RiscvPmpSemantics.
+
+End RiscvPmpIrisBase2.
